1) proving forward-simulation of sb_trans. Given a deterministic opsem, forward-simulation also implies backward-simulation. This proof requires a simulation relation over registers and memory states, which is a relation different from the injection and extension relations of CompCert memory model, because it allows possibly more blocks in a transformed program.
We need this relation because SoftBound uses additional memory blocks to
keep track meta data. This makes back-simulation failed: for example,
given a
  inttoptr ((i32 42) to i32*)
42 could be a valid address in those additional blocks of a transformed
program, but not a valid address of its original one.

2) fixed a bug of llvm bindings: should use Int64_val to convert Caml
value to a unsiged long long.

3) One more case for an inttoptr constant expression



git-svn-id: https://webdav.seas.upenn.edu/svn/sol/vol@2869 eef5ea85-cc2e-0410-bd84-0fae1f012da8

src/SoftBound/main.ml
@@ -5,7 +5,6 @@ open Llvm
 open Trace
 
 let main in_filename =
-
   let ic = global_context () in
   let imbuf = MemoryBuffer.of_file in_filename in
   let im = Llvm_bitreader.parse_bitcode ic imbuf in
@@ -17,13 +16,21 @@ let main in_filename =
   (if !Globalstates.debug then Coq_pretty_printer.travel_module coqim);
 
   (match SBpass.trans_module coqim with
-    | Some coqom -> Coq_pretty_printer.travel_module coqom
+    | Some coqom -> 
+        Coq_pretty_printer.travel_module coqom;
+(*
+        let om = Coq2llvm2.translate_module coqom in
+        (* write the module to a file *)
+        if not (Llvm_bitwriter.write_bitcode_file om out_filename) then 
+          exit 1
+*)
     | None -> failwith "failed");
 
   SlotTracker.dispose ist;
   dispose_module im
 
 let () = match Sys.argv with
-  | [| _; "-d" ; in_filename |] -> Globalstates.debug := true; main in_filename
+  | [| _; "-d" ; in_filename |] -> 
+       Globalstates.debug := true; main in_filename
   | [| _; in_filename |] -> main in_filename
   | _ -> main "Input.bc"
