src/SoftBound/sb_trans.v
@@ -17,6 +17,8 @@ Require Import monad.
 Require Import Metatheory.
 Require Import Znumtheory.
 Require Import sb_def.
+Require Import symexe_def.
+Require Import sb_tactic.
 
 Module SBpass.
 
@@ -164,6 +166,23 @@ Definition prop_metadata (ex_ids tmps:ids) rm c v1 id0 :=
   | _ => None
   end.
 
+Fixpoint trans_params (rm:rmap) (lp:params) : option params :=
+match lp with
+| nil => Some nil
+| (t0,v0) as p::lp' =>
+    match trans_params rm lp' with
+    | None => None
+    | Some lp2 =>
+      if isPointerTypB t0 then
+        match get_reg_metadata rm v0 with
+        | Some (bv0, ev0) =>
+            Some ((p8,bv0)::(p8,ev0)::lp2)
+        | _ => None
+        end
+      else Some lp2
+    end
+end.
+
 Definition trans_cmd (ex_ids tmps:ids) (addrb addre:id) (rm:rmap) (c:cmd) 
   : option (ids*ids*cmds) :=
 match c with 
@@ -174,7 +193,8 @@ match c with
       Some (ex_ids', tmp::tmps,
        c::
        insn_cast bid castop_bitcast (typ_pointer t1) (value_id id0) p8:: 
-       insn_gep tmp false (typ_pointer t1) (value_id id0) c1 :: 
+       insn_gep tmp false (typ_pointer t1) (value_id id0) 
+         (Cons_list_value v1 Nil_list_value) :: 
        insn_cast eid castop_bitcast (typ_pointer t1) (value_id tmp) p8:: 
        nil)
     | _ => None
@@ -192,11 +212,11 @@ match c with
           | Some (bid0, eid0) =>
               Some
                 (insn_call fake_id true false typ_void get_mmetadata_fn 
-                  ((p8,(value_id ptmp))::
+                  ((p8,v2)::
                    (p8,(value_id addrb))::
                    (p8,(value_id addre))::nil)::
-                 insn_load bid0 p8 (value_id addrb) Align.One::
-                 insn_load eid0 p8 (value_id addre) Align.One::   
+                 insn_load bid0 p8 (value_id addrb) Align.Zero::
+                 insn_load eid0 p8 (value_id addre) Align.Zero::   
                  nil)
           | None => None
           end
@@ -226,13 +246,13 @@ match c with
       let '(etmp,ex_ids) := mk_tmp ex_ids in
       let optcs := 
         if isPointerTypB t0 then
-          match lookupAL _ rm id0 with
-          | Some (bid0, eid0) =>
+          match get_reg_metadata rm v1 with
+          | Some (bv0, ev0) =>
               Some
                 (insn_call fake_id true false typ_void set_mmetadata_fn 
                   ((p8,(value_id ptmp))::
-                   (p8,(value_id bid0))::
-                   (p8,(value_id eid0))::nil)::
+                   (p8,bv0)::
+                   (p8,ev0)::nil)::
                  nil)
           | None => None
           end
@@ -289,6 +309,9 @@ match c with
       end
     else Some (ex_ids, tmps, [c])
 
+| insn_call id0 noret0 tailc0 rt fv lp =>
+    do lp' <- trans_params rm lp;
+    ret (ex_ids, tmps, [insn_call id0 noret0 tailc0 rt fv (lp++lp')])
 | _ => Some (ex_ids, tmps, [c])
 end.
 
@@ -377,12 +400,22 @@ match la with
       if isPointerTypB t0 then
         match (lookupAL _ rm id0) with
         | Some (bid0, eid0) => 
-            Some ((p8,bid0)::(p8,id0)::la2)
+            Some ((p8,bid0)::(p8,eid0)::la2)
         | _ => None
         end
       else Some la2
     end
 end.
+
+Definition insert_more_allocas (addrb addre:id) (b:block) : block :=
+let '(block_intro l1 ps1 cs1 tmn1) := b in
+block_intro l1 ps1
+  (insn_alloca addrb p8 
+    (value_const (const_int Size.ThirtyTwo (INTEGER.of_Z 32%Z 1%Z false))) 
+    Align.Zero::
+  insn_alloca addre p8 
+    (value_const (const_int Size.ThirtyTwo (INTEGER.of_Z 32%Z 1%Z false))) 
+    Align.Zero::cs1) tmn1.
 
 Definition trans_fdef (f:fdef) : option (rmap*ids*fdef) :=
 let '(fdef_intro (fheader_intro t fid la) bs) := f in
@@ -394,8 +427,11 @@ match gen_metedata_fdef ex_ids nil f with
         let '(addrb,ex_ids) := mk_tmp ex_ids in
         let '(addre,ex_ids) := mk_tmp ex_ids in
         match (trans_blocks ex_ids (addrb::addre::nil) addrb addre rm bs) with
-        | Some (ex_ids, tmps, bs') => 
-            Some (rm, tmps, fdef_intro (fheader_intro t fid (la++la')) bs')
+        | Some (ex_ids, tmps, b'::bs') => 
+            Some (rm, tmps, 
+              fdef_intro 
+                (fheader_intro t fid (la++la')) 
+                ((insert_more_allocas addrb addre b')::bs'))
         | _ => None
         end
     | _ => None
@@ -445,6 +481,364 @@ match ms with
     | _ => None
     end
 end.
+
+Definition reg_simulation (rm1:SoftBound.rmetadata) (rm2:rmap) (lc1 lc2:GVMap) 
+  : Prop :=
+(forall i0 gv, lookupAL _ lc1 i0 = Some gv -> lookupAL _ lc2 i0 = Some gv) /\
+(forall pid bgv egv, 
+  lookupAL _ rm1 pid = Some (SoftBound.mkMD bgv egv) -> 
+  exists bid, exists eid, 
+    lookupAL _ rm2 pid = Some (bid, eid) /\
+    lookupAL _ lc2 bid = Some bgv /\
+    lookupAL _ lc2 eid = Some egv) /\
+(forall pid bid eid bgv egv, 
+  lookupAL _ rm2 pid = Some (bid, eid) ->
+  lookupAL _ lc2 bid = Some bgv ->
+  lookupAL _ lc2 eid = Some egv ->
+  lookupAL _ rm1 pid = Some (SoftBound.mkMD bgv egv)).
+
+Definition sb_meminj (b:Values.block) : option (Values.block * Z) :=
+  Some (b, 0%Z).
+
+Definition sb_mem_inj (M M':mem) := Memory.Mem.mem_inj sb_meminj M M'.
+
+Definition mem_simulation TD (MM1:SoftBound.mmetadata) (Mem1 Mem2:mem) : Prop :=
+sb_mem_inj Mem1 Mem2 /\
+(forall lc gl b i bgv egv als lc' Mem1' tr addrb addre bid0 eid0 als' v, 
+  MM1 b i = Some (SoftBound.mkMD bgv egv) ->
+  getOperandValue TD Mem1 v lc gl = Some (ptr2GV TD (Vptr b i)) ->
+  SimpleSE.dbCmds TD gl lc als Mem1
+    (insn_call fake_id true false typ_void get_mmetadata_fn 
+       ((p8,v)::
+        (p8,(value_id addrb))::
+        (p8,(value_id addre))::nil)::
+     insn_load bid0 p8 (value_id addrb) Align.Zero::
+     insn_load eid0 p8 (value_id addre) Align.Zero::   
+     nil) lc' als' Mem1' tr ->
+  lookupAL _ lc' bid0 = Some bgv /\
+  lookupAL _ lc' bid0 = Some egv
+) /\
+(forall lc gl b i bgv egv als lc' Mem1' tr addrb addre bid0 eid0 als' v, 
+  getOperandValue TD Mem1 v lc gl = Some (ptr2GV TD (Vptr b i)) ->
+  SimpleSE.dbCmds TD gl lc als Mem1
+    (insn_call fake_id true false typ_void get_mmetadata_fn 
+       ((p8,v)::
+        (p8,(value_id addrb))::
+        (p8,(value_id addre))::nil)::
+     insn_load bid0 p8 (value_id addrb) Align.Zero::
+     insn_load eid0 p8 (value_id addre) Align.Zero::   
+     nil) lc' als' Mem1' tr ->
+  lookupAL _ lc' bid0 = Some bgv ->
+  lookupAL _ lc' bid0 = Some egv ->
+  MM1 b i = Some (SoftBound.mkMD bgv egv)
+).
+
+Fixpoint codom (rm:rmap) : atoms :=
+match rm with
+| nil => empty
+| (_,(bid,eid))::rm' => singleton bid `union` singleton eid `union` codom rm'
+end.
+
+Lemma reg_simulation__updateAddAL : forall rm1 rm2 lc1 lc2 i0 gv',
+  reg_simulation rm1 rm2 lc1 lc2 ->
+  i0 `notin` codom rm2 ->
+  reg_simulation rm1 rm2 (updateAddAL GenericValue lc1 i0 gv')
+    (updateAddAL GenericValue lc2 i0 gv').
+Admitted.
+
+Lemma simulation__BOP : forall rm rm2 lc lc2 TD MM Mem Mem2 gl bop0 sz0 v1 v2 
+                        gv3,
+  reg_simulation rm rm2 lc lc2 ->
+  mem_simulation TD MM Mem Mem2 ->
+  BOP TD Mem lc gl bop0 sz0 v1 v2 = ret gv3 ->
+  BOP TD Mem2 lc2 gl bop0 sz0 v1 v2 = ret gv3.
+Admitted.
+
+Lemma mem_simulation__malloc : forall TD MM Mem Mem2 tsz gn align0 Mem' mb,
+  mem_simulation TD MM Mem Mem2 ->
+  malloc TD Mem tsz gn align0 = ret (Mem', mb) ->
+  exists Mem2',
+    malloc TD Mem2 tsz gn align0 = ret (Mem2', mb) /\
+    mem_simulation TD MM Mem' Mem2'.
+Admitted.
+
+Lemma simulation__getOperandValue : forall rm rm2 lc lc2 TD MM Mem Mem2 gl v gv,
+  reg_simulation rm rm2 lc lc2 ->
+  mem_simulation TD MM Mem Mem2 ->
+  getOperandValue TD Mem v lc gl = ret gv ->
+  getOperandValue TD Mem2 v lc2 gl = ret gv.
+Admitted.
+
+Lemma mem_simulation__free : forall TD MM Mem Mem2 mptr0 Mem',
+  mem_simulation TD MM Mem Mem2 ->
+  free TD Mem mptr0 = ret Mem' ->
+  exists Mem2',
+    free TD Mem2 mptr0 = ret Mem2' /\
+    mem_simulation TD MM Mem' Mem2'.
+Admitted.
+
+Lemma trans_cmd__is__correct : forall c TD lc1 rm1 als gl Mem1 MM1 lc1' als' 
+    Mem1' MM1' tr lc2 Mem2 rm2 rm1' cs ex_ids tmps addrb addre ex_ids' tmps' r,  
+  getCmdID c `notin` codom rm2 ->
+  trans_cmd ex_ids tmps addrb addre rm2 c = Some (ex_ids', tmps', cs) ->
+  reg_simulation rm1 rm2 lc1 lc2 ->
+  mem_simulation TD MM1 Mem1 Mem2 ->
+  SoftBound.dbCmd TD gl lc1 rm1 als Mem1 MM1 c lc1' rm1' als' Mem1' MM1' tr r ->
+  exists lc2', exists Mem2',
+   SimpleSE.dbCmds TD gl lc2 als Mem2 cs lc2' als' Mem2' tr /\
+   reg_simulation rm1' rm2 lc1' lc2' /\
+   mem_simulation TD MM1' Mem1' Mem2'.
+Proof.
+  intros c TD lc1 rm1 als gl Mem1 MM1 lc1' als' Mem1' MM1' tr lc2 Mem2 rm2 rm1' 
+    cs ex_ids tmps addrb addre ex_ids' tmps' r Hnotin Htrans Hrsim Hmsim HdbCmd.
+  (sb_dbCmd_cases (destruct HdbCmd) Case); simpl in Htrans.
+
+Case "dbBop".
+  inv Htrans.
+  exists (updateAddAL GenericValue lc2 id0 gv3). exists Mem2. 
+  split.
+   assert (trace_nil = trace_app trace_nil trace_nil) as EQ. auto.
+   rewrite EQ.
+   eapply SimpleSE.dbCmds_cons; eauto.
+     apply SimpleSE.dbBop; eauto using simulation__BOP.
+  split; auto.
+    apply reg_simulation__updateAddAL; auto.
+
+admit. admit. admit. admit. admit. admit. admit.
+
+Case "dbMalloc".
+  remember (lookupAL (id * id) rm2 id0) as R1.
+  destruct R1; try solve [inversion Htrans].
+  destruct p as [bid eid].
+  remember (mk_tmp ex_ids) as R2.
+  destruct R2 as [tmp ex_ids''].
+  inv Htrans.
+  invert_prop_reg_metadata.
+  apply mem_simulation__malloc with (MM:=MM)(Mem2:=Mem2) in H1; auto.
+  destruct H1 as [Mem2' [H11 H12]].
+  exists 
+    (updateAddAL _ 
+      (updateAddAL _ 
+        (updateAddAL _ 
+          (updateAddAL GenericValue lc2 id0 (blk2GV TD mb))
+          bid (SoftBound.base2GV TD mb))
+        tmp (SoftBound.bound2GV TD mb tsz n))
+      eid (SoftBound.bound2GV TD mb tsz n)).
+  exists Mem2'.
+  split.
+    assert (trace_nil = trace_app trace_nil trace_nil) as EQ. auto.
+    rewrite EQ.
+    apply SimpleSE.dbCmds_cons with 
+      (lc2:=updateAddAL GenericValue lc2 id0 (blk2GV TD mb))(als2:=als)
+      (Mem2:=Mem2'); auto.
+      apply SimpleSE.dbMalloc with (gn:=gn)(tsz:=tsz); 
+        eauto using simulation__getOperandValue.
+    rewrite EQ.
+    apply SimpleSE.dbCmds_cons with 
+      (lc2:=updateAddAL _
+              (updateAddAL GenericValue lc2 id0 (blk2GV TD mb))
+              bid (SoftBound.base2GV TD mb)
+      )
+      (als2:=als)
+      (Mem2:=Mem2'); auto.
+      apply SimpleSE.dbCast; auto.
+        admit.
+    rewrite EQ.
+    apply SimpleSE.dbCmds_cons with 
+      (lc2:=updateAddAL _
+              (updateAddAL _
+                (updateAddAL GenericValue lc2 id0 (blk2GV TD mb))
+                 bid (SoftBound.base2GV TD mb))
+               tmp (SoftBound.bound2GV TD mb tsz n)
+      )
+      (als2:=als)
+      (Mem2:=Mem2'); auto.
+      apply SimpleSE.dbGEP with (mp:=blk2GV TD mb)(vidxs:=[gn]); auto.
+        admit. admit. admit.
+    rewrite EQ.
+    apply SimpleSE.dbCmds_cons with 
+      (lc2:=updateAddAL _
+              (updateAddAL _
+                (updateAddAL _
+                  (updateAddAL GenericValue lc2 id0 (blk2GV TD mb))
+                   bid (SoftBound.base2GV TD mb))
+                 tmp (SoftBound.bound2GV TD mb tsz n))
+               eid (SoftBound.bound2GV TD mb tsz n)
+      )
+      (als2:=als)
+      (Mem2:=Mem2'); auto.
+      apply SimpleSE.dbCast; auto.
+        admit.
+
+  split; auto.
+    admit.
+
+admit.    
+
+Case "dbFree".
+  inv Htrans.
+  apply mem_simulation__free with (MM:=MM)(Mem2:=Mem2) in H0; auto.
+  destruct H0 as [Mem2' [H01 H02]].
+  exists lc2. exists Mem2'. 
+  split.
+   assert (trace_nil = trace_app trace_nil trace_nil) as EQ. auto.
+   rewrite EQ.
+   eapply SimpleSE.dbCmds_cons; eauto.
+     apply SimpleSE.dbFree with (mptr:=mptr0); 
+       eauto using simulation__getOperandValue.
+  split; auto.
+
+admit. admit. admit.
+
+Case "dbLoad_nptr".
+  remember (get_reg_metadata rm2 vp) as R.
+  destruct R; try solve [inversion Htrans].
+  destruct p as [bv ev].
+  remember (mk_tmp ex_ids) as R1. 
+  destruct R1 as [ptmp ex_ids1].
+  remember (mk_tmp ex_ids1) as R2. 
+  destruct R2 as [btmp ex_ids2].
+  remember (mk_tmp ex_ids2) as R3. 
+  destruct R3 as [etmp ex_ids3].
+  remember (isPointerTypB t) as R4.
+  destruct R4.
+    unfold isPointerTyp in H3.
+    rewrite <- HeqR4 in H3.
+    contradict H3; auto.
+
+    inv Htrans.
+    admit.
+
+Case "dbLoad_ptr".
+  remember (get_reg_metadata rm2 vp) as R.
+  destruct R; try solve [inversion Htrans].
+  destruct p as [bv ev].
+  remember (mk_tmp ex_ids) as R1. 
+  destruct R1 as [ptmp ex_ids1].
+  remember (mk_tmp ex_ids1) as R2. 
+  destruct R2 as [btmp ex_ids2].
+  remember (mk_tmp ex_ids2) as R3. 
+  destruct R3 as [etmp ex_ids3].
+  remember (isPointerTypB t) as R4.
+  destruct R4.
+    remember (lookupAL (id * id) rm2 id0) as R5.
+    destruct R5; try solve [inversion Htrans].
+    destruct p as [bid0 eid0].
+    inv Htrans.
+    admit.
+
+    unfold isPointerTyp in H3.
+    rewrite <- HeqR4 in H3.
+    inversion H3.
+
+admit. admit. admit.
+
+Case "dbLoad_abort".
+  remember (get_reg_metadata rm2 vp) as R.
+  destruct R; try solve [inversion Htrans].
+  destruct p as [bv ev].
+  remember (mk_tmp ex_ids) as R1. 
+  destruct R1 as [ptmp ex_ids1].
+  remember (mk_tmp ex_ids1) as R2. 
+  destruct R2 as [btmp ex_ids2].
+  remember (mk_tmp ex_ids2) as R3. 
+  destruct R3 as [etmp ex_ids3].
+  remember (isPointerTypB t) as R4.
+  destruct R4.
+    remember (lookupAL (id * id) rm2 id0) as R5.
+    destruct R5; try solve [inversion Htrans].
+    destruct p as [bid0 eid0].
+    inv Htrans.
+    admit.
+
+    inv Htrans.
+    admit.
+
+Case "dbStore_nptr".
+  remember (get_reg_metadata rm2 vp) as R.
+  destruct R; try solve [inversion Htrans].
+  destruct p as [bv ev].
+  remember (mk_tmp ex_ids) as R1. 
+  destruct R1 as [ptmp ex_ids1].
+  remember (mk_tmp ex_ids1) as R2. 
+  destruct R2 as [btmp ex_ids2].
+  remember (mk_tmp ex_ids2) as R3. 
+  destruct R3 as [etmp ex_ids3].
+  remember (isPointerTypB t) as R4.
+  destruct R4.
+    unfold isPointerTyp in H4.
+    rewrite <- HeqR4 in H4.
+    contradict H4; auto.
+
+    inv Htrans.
+    admit.
+
+Case "dbStore_ptr".
+  remember (get_reg_metadata rm2 vp) as R.
+  destruct R; try solve [inversion Htrans].
+  destruct p as [bv ev].
+  remember (mk_tmp ex_ids) as R1. 
+  destruct R1 as [ptmp ex_ids1].
+  remember (mk_tmp ex_ids1) as R2. 
+  destruct R2 as [btmp ex_ids2].
+  remember (mk_tmp ex_ids2) as R3. 
+  destruct R3 as [etmp ex_ids3].
+  remember (isPointerTypB t) as R4.
+  destruct R4.
+    remember (get_reg_metadata rm2 v) as R5.
+    destruct R5; try solve [inversion Htrans].
+    destruct p as [bv0 ev0].
+    inv Htrans.
+    admit.
+
+    unfold isPointerTyp in H4.
+    rewrite <- HeqR4 in H4.
+    inversion H4.
+
+admit. admit. admit.
+
+Case "dbStore_abort".
+  remember (get_reg_metadata rm2 vp) as R.
+  destruct R; try solve [inversion Htrans].
+  destruct p as [bv ev].
+  remember (mk_tmp ex_ids) as R1. 
+  destruct R1 as [ptmp ex_ids1].
+  remember (mk_tmp ex_ids1) as R2. 
+  destruct R2 as [btmp ex_ids2].
+  remember (mk_tmp ex_ids2) as R3. 
+  destruct R3 as [etmp ex_ids3].
+  remember (isPointerTypB t) as R4.
+  destruct R4.
+    remember (get_reg_metadata rm2 v) as R5.
+    destruct R5; try solve [inversion Htrans].
+    destruct p as [bv0 ev0].
+    inv Htrans.
+    admit.
+
+    inv Htrans.
+    admit.
+
+Admitted.
+
+Fixpoint getCmdsIDs (cs:list cmd) : atoms :=
+match cs with
+| nil => empty
+| c::cs' => singleton (getCmdID c) `union` getCmdsIDs cs'
+end.
+
+Lemma trans_cmds__is__correct : forall cs TD lc1 rm1 als gl Mem1 MM1 lc1' als' 
+    Mem1' MM1' tr lc2 Mem2 rm2 rm1' cs' ex_ids tmps addrb addre ex_ids' tmps' r, 
+  AtomSetImpl.inter (getCmdsIDs cs) (codom rm2) [<=] empty ->
+  trans_cmds ex_ids tmps addrb addre rm2 cs = Some (ex_ids', tmps', cs') ->
+  reg_simulation rm1 rm2 lc1 lc2 ->
+  mem_simulation TD MM1 Mem1 Mem2 ->
+  SoftBound.dbCmds TD gl lc1 rm1 als Mem1 MM1 cs lc1' rm1' als' Mem1' MM1' tr r 
+    ->
+  exists lc2', exists Mem2',
+    SimpleSE.dbCmds TD gl lc2 als Mem2 cs' lc2' als' Mem2' tr /\
+    reg_simulation rm1' rm2 lc1' lc2' /\
+    mem_simulation TD MM1' Mem1' Mem2'.
+Admitted.
 
 End SBpass.
 
